theories/interop/wp_prims/length.v
@@ -22,29 +22,29 @@ Import mlanguage.
 
 Lemma length_correct e : |- wrap_prog e :: length_proto.
 Proof using.
-  iIntros (? ? ? ?) "H". unfold mprogwp. iNamed "H".
-  destruct bl as [tg vs0].
+  iIntros (? ? ? ?) "H". unfold mprogwp. iNamed "H". iPoseProof "Hpto" as "#Hpto".
   iSplit; first done.
   iIntros (Φ') "Hb Hcont". iApply wp_wrap_call; first done. cbn [snd].
   rewrite weakestpre.wp_unfold. rewrite /weakestpre.wp_pre.
   iIntros "%σ Hσ". cbn -[wrap_prog].
   SI_at_boundary. iNamed "HGC". SI_GC_agree. iNamed "HSI_block_level".
-  iDestruct "Hpto" as "(Hpto & Hptoacc)".
-  iPoseProof (lstore_own_elem_of with "GCζauth Hpto") as "%Helem".
-  iAssert ⌜∃ m', ζC ρc !! γ = Some (Bvblock (m', (tg, vs0)))⌝%I as "%Helem2".
+  iDestruct (lstore_own_head_of with "GCζauth Hpto") as %(blk&Helem&Hagr).
+  destruct blk as [(m&tg'&vs)| |]; try (cbn in *; congruence).
+  cbn in Hagr. simplify_eq.
+  iAssert ⌜∃ m', ζC ρc !! γ = Some (Bvblock (m', (tg, vs)))⌝%I as "%Helem2".
   1: { iPureIntro.
        eapply freeze_lstore_lookup_backwards in Helem as (?&Hfrz&?); eauto.
        inversion Hfrz; simplify_eq; eauto. }
   destruct Helem2 as [m' Helem2].
 
   iApply wp_pre_cases_c_prim; [done..|].
-  iExists (λ '(e', σ'), e' = WrSE (ExprV #(length vs0)) ∧ σ' = CState ρc mem).
+  iExists (λ '(e', σ'), e' = WrSE (ExprV #(length vs)) ∧ σ' = CState ρc mem).
   iSplit. { iPureIntro; econstructor; eauto. }
   iIntros (? ? ? (? & ?)); simplify_eq.
   do 3 iModIntro. iFrame. iSplitL "SIinit". { iExists false. iFrame. }
   iApply wp_value; first done.
   iApply "Hcont". iFrame.
-  iApply ("Cont" with "[-Hpto Hptoacc] [$Hpto $Hptoacc]"); try done; [].
+  iApply ("Cont"); try done; [].
   rewrite /GC /named.
   do 5 iExists _. iFrame. iSplit; last done.
   iExists _. iFrame. iPureIntro; split_and!; done.
